wip

LeanSubst/Basic.lean
@@ -1,4 +1,5 @@
 
+import Lean.Elab.Term
 import Lilac
 open Lilac
 
@@ -8,6 +9,32 @@ universe u
 
 universe u1 u2 u3
 variable {S : Type u1} {T : Type u2} {U : Type u3}
+variable {V : List (Type u1)}
+
+namespace Subst.Syntax
+  open Lean.Elab.Term
+
+  open Lean in
+  def MetaM.promote {α} (x : Meta.MetaM α) : Elab.Term.TermElabM α := x
+
+  def form_list : List Lean.Expr -> TermElabM (Lean.TSyntax `term)
+  | [] => `(List.nil)
+  | .cons x xs => do
+    let xs' <- form_list xs
+    `(List.cons $(<- exprToSyntax x) $xs')
+
+  def form_prod : List Lean.Expr -> TermElabM (Lean.TSyntax `term)
+  | [] => `(ULift.up Unit.unit)
+  | .cons x xs => do
+    let xs' <- form_prod xs
+    `(Prod.mk $(<- exprToSyntax x) $xs')
+
+  def get_ty_arg (e : TermElabM Lean.Expr) : TermElabM Lean.Expr := do
+    let e <- e
+    match e with
+    | .app _ ty => pure ty
+    | _ => Lean.Elab.throwUnsupportedSyntax
+end Subst.Syntax
 
 set_option linter.unusedVariables false in
 abbrev Var (T : Type u2) := Nat
@@ -16,47 +43,36 @@ structure Ren (T : Type u2) where
   act : Var T -> Var T
 
 @[simp]
-def List.RenMapType (S : Type u) : List (Type u) -> Type u
-| [] => S
-| .cons x xs => Ren x -> List.RenMapType S xs
+def List.Tuple (F : Type u1 -> Type u2) : List (Type u1) -> Type u2
+| [] => ULift Unit
+| .cons x xs => F x × List.Tuple F xs
 
 class RenMap (S : Type u) (V : List (Type u)) where
-  rmap : List.RenMapType (S -> S) V
+  rmap : List.Tuple Ren V -> S -> S
 
 export RenMap (rmap)
-
-def test1 : Ren Nat -> Nat -> Nat := sorry
-
-instance : RenMap Nat [Nat] where
-  rmap := test1
-
-def test2 : Ren Nat -> Ren Bool -> Nat -> Nat := sorry
-
-instance : RenMap Nat [Nat, Bool] where
-  rmap := test2
-
-theorem test3 {r1 : Ren Nat} {r2 : Ren Bool} {x : Nat} : @rmap _ [Nat, Bool] _ r1 r2 x = x := sorry
-
 
 macro:max (name := «term_⟨_,⟩») t:term noWs "⟨" r:term ",⟩" : term => `(rmap $r $t)
 syntax:max (name := «term_⟨_,+⟩») term noWs "⟨" term ,+ "⟩" : term
 
-open Lean in
-macro_rules
-  | `($t⟨ $elems,* ⟩) => do
-    let rec expand_ren_lit (i : Nat) (skip : Bool) (result : TSyntax `term) : MacroM Syntax := do
-      match i, skip with
-      | 0,     _     => pure result
-      | i + 1, true  => expand_ren_lit i false result
-      | i + 1, false => expand_ren_lit i true  (<- ``(Tuple.cons $(⟨elems.elemsAndSeps[i]!⟩) $result))
-    let size := elems.elemsAndSeps.size
-    let arg <- expand_ren_lit size (size % 2 == 0) (<- ``(Tuple.nil))
-    let arg : TSyntax `term := .mk arg
-    `(rmap $arg $t)
+open Lean.Meta in
+open Lean.Elab.Term in
+open Subst.Syntax in
+elab_rules <= expected
+| `($t⟨ $elems,* ⟩) => do
+  let elems <- List.mapM id $ elems.getElems.foldl (λ acc t => elabTerm t none :: acc) []
+  let elems_ty <- List.mapM id $ elems.map inferType |> List.map MetaM.promote |> List.map get_ty_arg
+  let list_ann <- form_list elems_ty.reverse
+  let elems_stx <- form_prod elems.reverse
+  let stx : TermElabM Lean.Syntax := `(@rmap _ $list_ann _ $elems_stx $t)
+  let stx <- stx
+  elabTerm stx expected
 
 @[app_unexpander rmap]
 def unexpand_rmap : Lean.PrettyPrinter.Unexpander
-| `($_ $r $t) => `($t⟨$r⟩)
+| `($_ ($r1, $r2, {down := ()}) $t) => `($t⟨$r1, $r2⟩)
+| `($_ ($r1, $r2, $r3, {down := ()}) $t) => `($t⟨$r1, $r2, $r3⟩)
+| `($_ $r $t) => `($t⟨$r,⟩)
 | _ => throw ()
 
 inductive Action (T : Type u2) where
@@ -77,30 +93,48 @@ def Subst.act [SubstAction S T U] (σ : Subst S) : T -> U := SubstAction.act σ
 instance : SubstAction T Nat (Action T) where
   act := Subst.inner
 
-class SubstMap {n} (S : Type u2) (V : Vec (Type u2) n) where
-  smap : V -> S -> S
+class SubstMap (S : Type u2) (V : List (Type u2)) where
+  smap : List.Tuple Subst V -> S -> S
 
 export SubstMap (smap)
 
 macro:max (name := «term_[_,]») t:term noWs "[" σ:term ",]" : term => `(smap $σ $t)
 syntax:max (name := «term_[_,+]») term noWs "[" term ,+ "]" : term
 
-open Lean in
-macro_rules
-  | `($t[ $elems,* ]) => do
-    let rec expand_subst_lit (i : Nat) (skip : Bool) (result : TSyntax `term) : MacroM Syntax := do
-      match i, skip with
-      | 0,     _     => pure result
-      | i + 1, true  => expand_subst_lit i false result
-      | i + 1, false => expand_subst_lit i true  (<- ``(Tuple.cons $(⟨elems.elemsAndSeps[i]!⟩) $result))
-    let size := elems.elemsAndSeps.size
-    let arg <- expand_subst_lit size (size % 2 == 0) (<- ``(Tuple.nil))
-    let arg : TSyntax `term := .mk arg
-    `(smap $arg $t)
+open Lean.Meta in
+open Lean.Elab.Term in
+open Subst.Syntax in
+elab_rules <= expected
+| `($t[ $elems,* ]) => do
+  let elems <- List.mapM id $ elems.getElems.foldl (λ acc t => elabTerm t none :: acc) []
+  let elems_ty <- List.mapM id $ elems.map inferType |> List.map MetaM.promote |> List.map get_ty_arg
+  let list_ann <- form_list elems_ty.reverse
+  let elems_stx <- form_prod elems.reverse
+  let stx : TermElabM Lean.Syntax := `(@smap _ $list_ann _ $elems_stx $t)
+  let stx <- stx
+  elabTerm stx expected
 
 @[app_unexpander smap]
 def unexpand_smap : Lean.PrettyPrinter.Unexpander
-| `($_ $σ $t) => `($t[$σ])
+| `($_ ($σ1, $σ2, {down := ()}) $t) => `($t[$σ1, $σ2])
+| `($_ ($σ1, $σ2, $σ3, {down := ()}) $t) => `($t[$σ1, $σ2, $σ3])
+| `($_ $σ $t) => `($t[$σ,])
 | _ => throw ()
+
+
+def test1 : Subst Nat × ULift Unit -> Nat -> Nat := sorry
+
+instance : SubstMap Nat [Nat] where
+  smap := test1
+
+def test2 : Subst Nat × Subst Bool × ULift Unit -> Nat -> Nat := sorry
+
+instance : SubstMap Nat [Nat, Bool] where
+  smap := test2
+
+theorem test3 {r1 : Subst Nat} {r2 : Subst Bool} {x : Nat} : x[r1, r2] = x := sorry
+
+theorem test4 [SubstMap S V] {v : List.Tuple Subst V} {x : S} : x[v,] = x := sorry
+
 
 end LeanSubst
