LeanSubst/Class.lean
@@ -7,9 +7,9 @@ namespace LeanSubst
 
 universe u1 u2 u3
 variable {S : Type u1} {T : Type u2} {U : Type u3}
-variable {n : Nat} {V : Vec (Type u) n}
+variable {n : Nat} {V : Vec (Type u2) n}
 
-class RenMapId (S : Type u1) (T : Type u2) [RenMap S T] where
+class RenMapId (S : Type u1) (T : Type u2) [RenMap S V] where
   apply_id {s : S} : s⟨Ren.id T⟩ = s
 
 class RenMapCompose (S : Type u1) (T : Type u2) [RenMap S T] where
